lakefile.lean
@@ -15,3 +15,7 @@ lean_exe tv where
 lean_exe testAdbc where
   root := `TestAdbc
   moreLinkArgs := #["c/libadbcshim.a", "-Wl,--allow-shlib-undefined"]
+
+lean_exe test where
+  root := `Test
+  moreLinkArgs := #["c/libtermshim.a", "c/libadbcshim.a", "-L/usr/local/lib", "-ltermbox2", "-Wl,--allow-shlib-undefined"]
